barrier/tests.v
@@ -32,16 +32,16 @@ End ParamTests.
 Module LiftingTests.
   (* TODO RJ: Some syntactic sugar for language expressions would be nice. *)
   Definition e3 := Load (Var 0).
-  Definition e2 := Seq (Store (Var 0) (Plus (Load (Var 0)) (LitNat 1))) e3.
+  Definition e2 := Seq (Store (Var 0) (Plus (Load $ Var 0) (LitNat 1))) e3.
   Definition e := Let (Alloc (LitNat 1)) e2.
   Goal ∀ σ E, (ownP (Σ:=Σ) σ) ⊑ (wp (Σ:=Σ) E e (λ v, ■(v = LitNatV 2))).
   Proof.
     move=> σ E. rewrite /e.
-    rewrite -(wp_bind _ _ (LetCtx EmptyCtx e2)). rewrite -wp_alloc_pst; last done.
+    rewrite -wp_let. rewrite -wp_alloc_pst; last done.
     apply sep_intro_True_r; first done.
     rewrite -later_intro. apply forall_intro=>l.
     apply wand_intro_l. rewrite right_id. apply const_elim_l; move=>_.
-    rewrite -wp_lam -later_intro. asimpl.
+    rewrite -later_intro. asimpl.
     rewrite -(wp_bind _ _ (SeqCtx (StoreRCtx (LocV _)
                                    (PlusLCtx EmptyCtx _)) (Load (Loc _)))).
     rewrite -wp_load_pst; first (apply sep_intro_True_r; first done); last first.
@@ -54,10 +54,48 @@ Module LiftingTests.
     { apply: lookup_insert. }
     { reflexivity. }
     rewrite -later_intro. apply wand_intro_l. rewrite right_id.
-    rewrite -wp_lam -later_intro. asimpl.
+    rewrite -wp_lam // -later_intro. asimpl.
     rewrite -wp_load_pst; first (apply sep_intro_True_r; first done); last first.
     { apply: lookup_insert. }
     rewrite -later_intro. apply wand_intro_l. rewrite right_id.
     by apply const_intro.
+  Qed.
+
+  Import Nat.
+
+  Definition Lt e1 e2 := Le (Plus e1 $ LitNat 1) e2.
+  Definition FindPred' n1 Sn1 n2 f := If (Lt Sn1 n2)
+                                      (App f Sn1)
+                                      n1.
+  Definition FindPred n2 := Rec (Let (Plus (Var 1) (LitNat 1))
+                                     (FindPred' (Var 2) (Var 0) n2.[ren(+3)] (Var 1))).
+  Lemma FindPred_spec n1 n2 E Q :
+    (■(n1 < n2) ∧ Q (LitNatV $ pred n2)) ⊑
+       wp (Σ:=Σ) E (App (FindPred (LitNat n2)) (LitNat n1)) Q.
+  Proof.
+    revert n1. apply löb_all_1=>n1.
+    rewrite -wp_rec //. asimpl.
+    (* Get rid of the ▷ in the premise. *)
+    etransitivity; first (etransitivity; last eapply equiv_spec, later_and).
+    { apply and_mono; first done. by rewrite -later_intro. }
+    apply later_mono.
+    (* Go on. *)
+    rewrite -(wp_let _ (FindPred' (LitNat n1) (Var 0) (LitNat n2) (FindPred $ LitNat n2))).
+    rewrite -wp_plus. asimpl.
+    rewrite -(wp_bind _ _ (CaseCtx EmptyCtx _ _)).
+    rewrite -(wp_bind _ _ (LeLCtx EmptyCtx _)).
+    rewrite -wp_plus -!later_intro. simpl.
+    assert (Decision (S n1 + 1 ≤ n2)) as Hn12 by apply _.
+    destruct Hn12 as [Hle|Hgt].
+    - rewrite -wp_le_true /= //. rewrite -wp_case_inl //.
+      rewrite -!later_intro. asimpl.
+      rewrite (forall_elim _ (S n1)).
+      eapply impl_elim; first by eapply and_elim_l. apply and_intro.
+      + apply const_intro; omega.
+      + by rewrite !and_elim_r.
+    - rewrite -wp_le_false; last by omega.
+      rewrite -wp_case_inr // -!later_intro -wp_value' //.
+      rewrite and_elim_r. apply const_elim_l=>Hle.
+      assert (Heq: n1 = pred n2) by omega. by subst n1=>{Hle Hgt}.
   Qed.
 End LiftingTests.
